src/Examples/Interval/CallString/Example_Interval_DG_CallString.thy
@@ -55,7 +55,7 @@ text \<open>The root context is \<^const>\<open>cfg_entry\<close> \<open>twice_c
 definition twice_cs_eqs :: "(pp \<times> cfg_node, gk_cs, (ivl exec_dg_st, ivl exec_dg_st) dg_state) eqsT" where
   "twice_cs_eqs =
      side_cfg_T_eff_keyed_seed_dg intra_predecessor_list (\<lambda>_. GlobalCS) route_cs
-       (routed_cmb Spoly GlobalCS) (routed_extra twice_cfg Spoly SeedCS GlobalCS)
+      (routed_cmb Spoly GlobalCS SeedCS) (routed_extra SeedCS GlobalCS)
        twice_cfg Spoly bot cinit_ivl_st (restrict_global_resolved_q cinit_ivl_st)"
 
 definition twice_cs_sol ::
@@ -153,45 +153,21 @@ lemma dg_tree_st_commute_frame_read_cs:
                 dep_aux_def bot_fun_def)
 
 lemma dg_tree_st_commute_routed_cmb_cs:
-  "dg_tree_st_commute_for twice_gs env (routed_cmb Spoly GlobalCS route_cs ctx ca cc ex)
-                          (routed_cmb Sabs GlobalCS route_cs ctx ca cc ex)"
+  "dg_tree_st_commute_for twice_gs env (routed_cmb Spoly GlobalCS SeedCS route_cs ctx ca cc ex)
+                          (routed_cmb Sabs GlobalCS SeedCS route_cs ctx ca cc ex)"
   unfolding routed_cmb_def Let_def
   by (cases ca)
      (simp_all add: dg_tree_st_commute_for_def fun_of_dg_st_for_simps fun_of_exec_dg_st_for_bot o_def
                     route_cs_def dgs_combine_fst_commute_gen dgs_combine_snd_commute_gen
+                    dgs_enter_fst_commute_gen dgs_enter_snd_commute_gen fun_of_dg_st_for_sup
                     dep_aux_def bot_fun_def fun_upd_apply fun_eq_iff)
-
-lemma dg_tree_st_commute_routed_enter_pub_cs:
-  "dg_tree_st_commute_for twice_gs env
-     (with_call a (\<lambda>dst fs as. do {
-        entry_state \<leftarrow> read_local (v, ctx);
-        globals_state \<leftarrow> read_global GlobalCS;
-        publish_global GlobalCS (enter_global Spoly fs as (locals entry_state) (globs globals_state));
-        publish_seed (SeedCS w (route_cs v ctx (locals entry_state) a))
-          (enter_local Spoly fs as (locals entry_state) (globs globals_state));
-        answer_local bot
-      }))
-     (with_call a (\<lambda>dst fs as. do {
-        entry_state \<leftarrow> read_local (v, ctx);
-        globals_state \<leftarrow> read_global GlobalCS;
-        publish_global GlobalCS (enter_global Sabs fs as (locals entry_state) (globs globals_state));
-        publish_seed (SeedCS w (route_cs v ctx (locals entry_state) a))
-          (enter_local Sabs fs as (locals entry_state) (globs globals_state));
-        answer_local bot
-      }))"
-  by (cases a)
-     (simp add: dg_tree_st_commute_for_def fun_of_dg_st_for_simps fun_of_exec_dg_st_for_bot o_def
-                route_cs_def dgs_enter_fst_commute_gen dgs_enter_snd_commute_gen
-                dep_aux_def bot_fun_def fun_upd_apply fun_eq_iff)
 
 lemma hextra_commute_routed_cs:
   "list_all2 (dg_tree_st_commute_for twice_gs env)
-     (routed_extra twice_cfg Spoly SeedCS GlobalCS route_cs ctx w)
-     (routed_extra twice_cfg Sabs SeedCS GlobalCS route_cs ctx w)"
+     (routed_extra SeedCS GlobalCS route_cs ctx w)
+     (routed_extra SeedCS GlobalCS route_cs ctx w)"
   unfolding routed_extra_def Let_def
-  by (auto simp: list_all2_appendI list_all2_map1 list_all2_map2 list_all2_refl split_beta
-                 dg_tree_st_commute_frame_read_cs dg_tree_st_commute_routed_enter_pub_cs
-           split: cfg_node.split)
+  by (auto simp: dg_tree_st_commute_frame_read_cs split: cfg_node.split)
 
 lemma twice_cs_solve_dom:
   "TD_side_warrowing_apinis_Interp.solve_dom TYPE(gk_cs) TYPE((ivl exec_dg_st, ivl exec_dg_st) dg_state)
@@ -211,14 +187,14 @@ lemma twice_cs_pp_st:
 theorem twice_cs_pp_abs:
   "part_post_solution
      (side_cfg_T_eff_keyed_seed_dg intra_predecessor_list (\<lambda>_. GlobalCS) route_cs
-        (routed_cmb Sabs GlobalCS) (routed_extra twice_cfg Sabs SeedCS GlobalCS) twice_cfg Sabs
+        (routed_cmb Sabs GlobalCS SeedCS) (routed_extra SeedCS GlobalCS) twice_cfg Sabs
         (fun_of_exec_dg_st_for twice_gs (bot::ivl exec_dg_st)) (fun_of_exec_dg_st_for twice_gs cinit_ivl_st)
         (fun_of_exec_dg_st_for twice_gs (restrict_global_resolved_q cinit_ivl_st)))
      (cfg_exit twice_cfg, cfg_entry twice_cfg) (fun_of_dg_st_for twice_gs \<circ> snd twice_cs_sol) (fst twice_cs_sol)"
 proof -
   have pp': "part_post_solution
        (side_cfg_T_eff_keyed_seed_dg intra_predecessor_list (\<lambda>_. GlobalCS) route_cs
-          (routed_cmb Spoly GlobalCS) (routed_extra twice_cfg Spoly SeedCS GlobalCS) twice_cfg Spoly
+          (routed_cmb Spoly GlobalCS SeedCS) (routed_extra SeedCS GlobalCS) twice_cfg Spoly
           bot cinit_ivl_st (restrict_global_resolved_q cinit_ivl_st))
        (cfg_exit twice_cfg, cfg_entry twice_cfg) (snd twice_cs_sol) (fst twice_cs_sol)"
     using twice_cs_pp_st unfolding twice_cs_eqs_def by simp
@@ -230,9 +206,9 @@ proof -
     by (rule part_post_solution_seed_dg_st_to_abs_for
           [where gs = twice_gs and pred_sel = intra_predecessor_list and gkey = "\<lambda>_. GlobalCS"
              and route_st = route_cs and route_abs = route_cs
-             and cmb_st = "routed_cmb Spoly GlobalCS" and cmb_abs = "routed_cmb Sabs GlobalCS"
-             and extra_st = "routed_extra twice_cfg Spoly SeedCS GlobalCS"
-             and extra_abs = "routed_extra twice_cfg Sabs SeedCS GlobalCS"
+             and cmb_st = "routed_cmb Spoly GlobalCS SeedCS" and cmb_abs = "routed_cmb Sabs GlobalCS SeedCS"
+             and extra_st = "routed_extra SeedCS GlobalCS"
+             and extra_abs = "routed_extra SeedCS GlobalCS"
              and g = twice_cfg and S_st = Spoly and S_abs = Sabs,
            OF ivl_Hstep_cs route_cs_commute dg_tree_st_commute_routed_cmb_cs
               hextra_commute_routed_cs pp'])
@@ -252,7 +228,7 @@ abbreviation sigma_cs :: "pp \<times> cfg_node + gk_cs \<Rightarrow> (ivl abs_st
 
 abbreviation gen_cs_abs :: "(pp \<times> cfg_node, gk_cs, (ivl abs_state, ivl abs_state) dg_state) eqsT" where
   "gen_cs_abs \<equiv> side_cfg_T_eff_keyed_seed_dg intra_predecessor_list (\<lambda>_. GlobalCS) route_cs
-       (routed_cmb Sabs GlobalCS) (routed_extra twice_cfg Sabs SeedCS GlobalCS) twice_cfg Sabs
+       (routed_cmb Sabs GlobalCS SeedCS) (routed_extra SeedCS GlobalCS) twice_cfg Sabs
        (fun_of_exec_dg_st_for twice_gs (bot::ivl exec_dg_st)) (fun_of_exec_dg_st_for twice_gs cinit_ivl_st)
        (fun_of_exec_dg_st_for twice_gs (restrict_global_resolved_q cinit_ivl_st))"
 
@@ -321,7 +297,7 @@ text \<open>\<open>ivl_dg_for\<close> (\<open>Example_Interval_DG_Ctx_Sound\<clo
   \<open>dg_ctx_activation\<close> inherits from it discharge automatically below.\<close>
 
 interpretation twice_cs_dg: dg_ctx_activation Sabs twice_gs twice_cfg GlobalCS route_cs
-    "routed_cmb Sabs GlobalCS" "routed_extra twice_cfg Sabs SeedCS GlobalCS"
+    "routed_cmb Sabs GlobalCS SeedCS" "routed_extra SeedCS GlobalCS"
     "fun_of_exec_dg_st_for twice_gs (bot::ivl exec_dg_st)" "fun_of_exec_dg_st_for twice_gs cinit_ivl_st"
     "fun_of_exec_dg_st_for twice_gs (restrict_global_resolved_q cinit_ivl_st)"
     sigma_cs "fst twice_cs_sol" "(cfg_exit twice_cfg, cfg_entry twice_cfg)" ivl_ctx_sg_cs
@@ -330,7 +306,7 @@ proof unfold_locales
 next
   show "part_post_solution
           (side_cfg_T_eff_keyed_seed_dg intra_predecessor_list (\<lambda>_. GlobalCS) route_cs
-             (routed_cmb Sabs GlobalCS) (routed_extra twice_cfg Sabs SeedCS GlobalCS) twice_cfg Sabs
+             (routed_cmb Sabs GlobalCS SeedCS) (routed_extra SeedCS GlobalCS) twice_cfg Sabs
              (fun_of_exec_dg_st_for twice_gs (bot::ivl exec_dg_st)) (fun_of_exec_dg_st_for twice_gs cinit_ivl_st)
              (fun_of_exec_dg_st_for twice_gs (restrict_global_resolved_q cinit_ivl_st)))
           (cfg_exit twice_cfg, cfg_entry twice_cfg) sigma_cs (fst twice_cs_sol)"
