src/Examples/Interval/CallString/Example_Interval_DG_CallString_K1.thy
@@ -99,7 +99,7 @@ subsection \<open>The routed equation system and its computed solution\<close>
 definition nest_1_eqs :: "(pp \<times> cfg_node list, gk_1, (ivl exec_dg_st, ivl exec_dg_st) dg_state) eqsT" where
   "nest_1_eqs =
      side_cfg_T_eff_keyed_seed_dg intra_predecessor_list (\<lambda>_. Global1) (cs_route 1)
-       (routed_cmb Spoly Global1) (routed_extra nest_cfg Spoly Seed1 Global1)
+      (routed_cmb Spoly Global1 Seed1) (routed_extra Seed1 Global1)
        nest_cfg Spoly bot cinit_ivl_st (restrict_global_resolved_q cinit_ivl_st)"
 
 definition nest_1_sol ::
@@ -242,45 +242,21 @@ lemma dg_tree_st_commute_frame_read_1:
                 dep_aux_def bot_fun_def)
 
 lemma dg_tree_st_commute_routed_cmb_1:
-  "dg_tree_st_commute_for nest_gs env (routed_cmb Spoly Global1 (cs_route 1) ctx ca cc ex)
-                          (routed_cmb Sabs Global1 (cs_route 1) ctx ca cc ex)"
+  "dg_tree_st_commute_for nest_gs env (routed_cmb Spoly Global1 Seed1 (cs_route 1) ctx ca cc ex)
+                          (routed_cmb Sabs Global1 Seed1 (cs_route 1) ctx ca cc ex)"
   unfolding routed_cmb_def Let_def
   by (cases ca)
      (simp_all add: dg_tree_st_commute_for_def fun_of_dg_st_for_simps fun_of_exec_dg_st_for_bot o_def
                     cs_route_def dgs_combine_fst_commute_gen dgs_combine_snd_commute_gen
+                    dgs_enter_fst_commute_gen dgs_enter_snd_commute_gen fun_of_dg_st_for_sup
                     dep_aux_def bot_fun_def fun_upd_apply fun_eq_iff)
-
-lemma dg_tree_st_commute_routed_enter_pub_1:
-  "dg_tree_st_commute_for nest_gs env
-     (with_call a (\<lambda>dst fs as. do {
-        entry_state \<leftarrow> read_local (v, ctx);
-        globals_state \<leftarrow> read_global Global1;
-        publish_global Global1 (enter_global Spoly fs as (locals entry_state) (globs globals_state));
-        publish_seed (Seed1 w (cs_route 1 v ctx (locals entry_state) a))
-          (enter_local Spoly fs as (locals entry_state) (globs globals_state));
-        answer_local bot
-      }))
-     (with_call a (\<lambda>dst fs as. do {
-        entry_state \<leftarrow> read_local (v, ctx);
-        globals_state \<leftarrow> read_global Global1;
-        publish_global Global1 (enter_global Sabs fs as (locals entry_state) (globs globals_state));
-        publish_seed (Seed1 w (cs_route 1 v ctx (locals entry_state) a))
-          (enter_local Sabs fs as (locals entry_state) (globs globals_state));
-        answer_local bot
-      }))"
-  by (cases a)
-     (simp add: dg_tree_st_commute_for_def fun_of_dg_st_for_simps fun_of_exec_dg_st_for_bot o_def
-                cs_route_def dgs_enter_fst_commute_gen dgs_enter_snd_commute_gen
-                dep_aux_def bot_fun_def fun_upd_apply fun_eq_iff)
 
 lemma hextra_commute_routed_1:
   "list_all2 (dg_tree_st_commute_for nest_gs env)
-     (routed_extra nest_cfg Spoly Seed1 Global1 (cs_route 1) ctx w)
-     (routed_extra nest_cfg Sabs Seed1 Global1 (cs_route 1) ctx w)"
+     (routed_extra Seed1 Global1 (cs_route 1) ctx w)
+     (routed_extra Seed1 Global1 (cs_route 1) ctx w)"
   unfolding routed_extra_def Let_def
-  by (auto simp: list_all2_appendI list_all2_map1 list_all2_map2 list_all2_refl split_beta
-                 dg_tree_st_commute_frame_read_1 dg_tree_st_commute_routed_enter_pub_1
-           split: cfg_node.split)
+  by (auto simp: dg_tree_st_commute_frame_read_1 split: cfg_node.split)
 
 lemma nest_1_solve_dom:
   "TD_side_warrowing_apinis_Interp.solve_dom TYPE(gk_1) TYPE((ivl exec_dg_st, ivl exec_dg_st) dg_state)
@@ -300,13 +276,13 @@ lemma nest_1_pp_st:
 theorem nest_1_pp_abs:
   "part_post_solution
      (side_cfg_T_eff_keyed_seed_dg intra_predecessor_list (\<lambda>_. Global1) (cs_route 1)
-        (routed_cmb Sabs Global1) (routed_extra nest_cfg Sabs Seed1 Global1) nest_cfg Sabs
+       (routed_cmb Sabs Global1 Seed1) (routed_extra Seed1 Global1) nest_cfg Sabs
         (fun_of_exec_dg_st_for nest_gs (bot::ivl exec_dg_st)) (fun_of_exec_dg_st_for nest_gs cinit_ivl_st) (fun_of_exec_dg_st_for nest_gs (restrict_global_resolved_q cinit_ivl_st)))
      (cfg_exit nest_cfg, []) (fun_of_dg_st_for nest_gs \<circ> snd nest_1_sol) (fst nest_1_sol)"
 proof -
   have pp': "part_post_solution
        (side_cfg_T_eff_keyed_seed_dg intra_predecessor_list (\<lambda>_. Global1) (cs_route 1)
-          (routed_cmb Spoly Global1) (routed_extra nest_cfg Spoly Seed1 Global1) nest_cfg Spoly
+          (routed_cmb Spoly Global1 Seed1) (routed_extra Seed1 Global1) nest_cfg Spoly
           bot cinit_ivl_st (restrict_global_resolved_q cinit_ivl_st))
        (cfg_exit nest_cfg, []) (snd nest_1_sol) (fst nest_1_sol)"
     using nest_1_pp_st unfolding nest_1_eqs_def by simp
@@ -318,9 +294,9 @@ proof -
     by (rule part_post_solution_seed_dg_st_to_abs_for
           [where gs = nest_gs and pred_sel = intra_predecessor_list and gkey = "\<lambda>_. Global1"
              and route_st = "cs_route 1" and route_abs = "cs_route 1"
-             and cmb_st = "routed_cmb Spoly Global1" and cmb_abs = "routed_cmb Sabs Global1"
-             and extra_st = "routed_extra nest_cfg Spoly Seed1 Global1"
-             and extra_abs = "routed_extra nest_cfg Sabs Seed1 Global1"
+             and cmb_st = "routed_cmb Spoly Global1 Seed1" and cmb_abs = "routed_cmb Sabs Global1 Seed1"
+             and extra_st = "routed_extra Seed1 Global1"
+             and extra_abs = "routed_extra Seed1 Global1"
              and g = nest_cfg and S_st = Spoly and S_abs = Sabs,              OF ivl_Hstep_1 cs_route_indep_of_data dg_tree_st_commute_routed_cmb_1
               hextra_commute_routed_1 pp'])
 qed
@@ -332,7 +308,7 @@ abbreviation sigma_1 :: "pp \<times> cfg_node list + gk_1 \<Rightarrow> (ivl abs
 
 abbreviation gen_1_abs :: "(pp \<times> cfg_node list, gk_1, (ivl abs_state, ivl abs_state) dg_state) eqsT" where
   "gen_1_abs \<equiv> side_cfg_T_eff_keyed_seed_dg intra_predecessor_list (\<lambda>_. Global1) (cs_route 1)
-       (routed_cmb Sabs Global1) (routed_extra nest_cfg Sabs Seed1 Global1) nest_cfg Sabs
+       (routed_cmb Sabs Global1 Seed1) (routed_extra Seed1 Global1) nest_cfg Sabs
        (fun_of_exec_dg_st_for nest_gs (bot::ivl exec_dg_st)) (fun_of_exec_dg_st_for nest_gs cinit_ivl_st) (fun_of_exec_dg_st_for nest_gs (restrict_global_resolved_q cinit_ivl_st))"
 
 lemma pp_eq_bound_1:
@@ -393,7 +369,7 @@ interpretation ivl_dg_for: sound_dg_spec Sabs "gamma_unit nest_gs" nest_gs
   by (rule sound_dg_spec_unit_for[OF ivl_is_sound_transfer_for nest_reserved])
 
 interpretation nest_1_dg: dg_ctx_activation Sabs nest_gs nest_cfg Global1 "cs_route 1"
-    "routed_cmb Sabs Global1" "routed_extra nest_cfg Sabs Seed1 Global1"
+    "routed_cmb Sabs Global1 Seed1" "routed_extra Seed1 Global1"
     "fun_of_exec_dg_st_for nest_gs (bot::ivl exec_dg_st)" "fun_of_exec_dg_st_for nest_gs cinit_ivl_st" "fun_of_exec_dg_st_for nest_gs (restrict_global_resolved_q cinit_ivl_st)"
     sigma_1 "fst nest_1_sol" "(cfg_exit nest_cfg, [])" ivl_ctx_sg_1
 proof unfold_locales
@@ -401,7 +377,7 @@ proof unfold_locales
 next
   show "part_post_solution
           (side_cfg_T_eff_keyed_seed_dg intra_predecessor_list (\<lambda>_. Global1) (cs_route 1)
-             (routed_cmb Sabs Global1) (routed_extra nest_cfg Sabs Seed1 Global1) nest_cfg Sabs
+             (routed_cmb Sabs Global1 Seed1) (routed_extra Seed1 Global1) nest_cfg Sabs
              (fun_of_exec_dg_st_for nest_gs (bot::ivl exec_dg_st)) (fun_of_exec_dg_st_for nest_gs cinit_ivl_st)
              (fun_of_exec_dg_st_for nest_gs (restrict_global_resolved_q cinit_ivl_st)))
           (cfg_exit nest_cfg, []) sigma_1 (fst nest_1_sol)"
